some allocation

examples/csl/SL.Actions.fst
@@ -27,3 +27,15 @@ let frame_write_wp (#a:Type) (r:ref a) (v:a) : st_wp unit =
 assume
 val ( := ) (#a:Type) (r:ref a) (v:a)
   :STATE unit (frame_write_wp r v)
+
+
+let alloc_wp (#a:Type) (v:a) : st_wp (ref a) =
+  (fun post m0 -> forall (r:ref a). m0 == emp  /\ post r (r |> v))
+
+unfold
+let frame_alloc_wp (#a:Type) (v:a) : st_wp (ref a) =
+   fun post m0 -> frame_wp (with_fp [] <| alloc_wp v) (frame_post post) m0
+
+assume
+val alloc (#a:Type) (v:a)
+  :STATE (ref a) (frame_alloc_wp v)
